Progress with invariant; had to add conservation
Fix statement

Comment out insanity

PoS/InvCliqueTopology.v
@@ -28,7 +28,18 @@ Definition GSyncing_clique w :=
    largest_chain w bc,
 
    (* Clique topology *)
-   forall n', holds n' w (fun st => peers st =i dom (localState w)) &
+   forall n', holds n' w (fun st => {subset (dom (localState w)) <= peers st}) &
+
+   (*
+   (* Conservation of blocks in clique topology *)
+   [/\ forall n1, holds n1 w (fun st => forall b, b ∈ (blockTree st) ->
+        forall n2, holds n2 w (fun st' => b ∈ (blockTree st') \/ b \in blocksFor n2 w)) &
+
+        forall p, p \in inFlightMsgs w -> forall b, msg p = BlockMsg b ->
+          exists n' st', find n' (localState w) = Some st' /\
+                    holds n' w (fun st => b ∈ (blockTree st))
+   ] &
+   *)
 
    (* Applying blocks in flight will induce either the canonical
       chain or a smaller one. *)
@@ -36,20 +47,170 @@ Definition GSyncing_clique w :=
       holds n' w (fun st =>
        bc = btChain (foldl btExtend (blockTree st) (blocksFor n' w)))].
 
-Definition BT_clique_inv (w : World) :=
+Definition clique_inv (w : World) :=
   Coh w /\ [\/ GStable w | GSyncing_clique w].
 
 Lemma clique_eventual_consensus w n :
-  BT_clique_inv w -> blocksFor n w == [::] ->
+  clique_inv w -> blocksFor n w == [::] ->
   holds n w (fun st => exists bc, (has_chain bc st) /\ largest_chain w bc).
 Proof.
-case=>C; case=>[H|[bc][can_n][H1 H2 H3 H4]] Na st Fw.
+case=>C; case=>[H|[bc][can_n][H1 H2 H3 H5]] Na st Fw.
 - case: H=>cE[bc]H; exists bc; split=>//; first by move:(H _ _ Fw).
   move=>n' bc' st' Fw'/eqP Z.
   by move: (H n' _ Fw')=>/eqP; rewrite Z=>->; left.
 exists bc; split=>//.
-move/eqP:Na=>Na. 
-by rewrite (H4 n _ Fw); rewrite Na/= /has_chain eqxx.
+move/eqP:Na=>Na.
+by rewrite (H5 n _ Fw); rewrite Na/= /has_chain eqxx.
 Qed.
 
+Ltac NBlockMsg_dest_bt q st p b Msg H :=
+  (have: (forall b, msg p != BlockMsg b) by move=>b; rewrite Msg)=>H;
+  move: (procMsg_non_block_nc_blockTree st (ts q) H).
+
+Ltac NBlockMsg_dest_btChain q st p b Msg P H :=
+  (have: (forall b, msg p != BlockMsg b) by move=>b; rewrite Msg)=>H;
+  move: (procMsg_non_block_nc_btChain st (ts q) H);
+  rewrite/has_chain Msg P /==><-.
+
+Ltac BlockMsg_dest q st b iF P Msg :=
+  rewrite [procMsg _ _ _] surjective_pairing in P; case: P=><- _;
+  rewrite/has_chain (procMsg_block_btExtend_btChain st b (ts q));
+  move: (b_in_blocksFor iF Msg)=>iB.
+
+Ltac simplw w :=
+have: ((let (_, inFlightMsgs, _) := w in inFlightMsgs) = inFlightMsgs w) by [];
+have: ((let (localState, _, _) := w in localState) = localState w) by [].
+
 (* TODO: Now the inductive version. *)
+Lemma clique_inv_step w w' q :
+  clique_inv w -> system_step w w' q -> clique_inv w'.
+Proof.
+move=>Iw S; rewrite/clique_inv; split; first by apply (Coh_step S).
+case: S; first by elim; move=>_ <-; apply Iw.
+(* Deliver *)
+move=> p st Cw. assert (Cw' := Cw). case Cw'=>[c1 c2 c3 c4 c5] Al iF F;
+case: Iw=>_ [GStabW|GSyncW].
+- by case GStabW=>noPackets; contradict iF; rewrite noPackets.
+- case: GSyncW=>can_bc [can_n] [] HHold HGt HCliq (*[HCon1 HCon2]*) HExt.
+  move=>P; assert (P' := P).
+  move: P; case P: (procMsg _ _ _)=>[stPm ms]; move=>->; right.
+  (* The canonical chain is guaranteed to remain the same for any Msg *)
+  exists can_bc, can_n; split.
+
+  (* can_n still retains can_bc *)
+  + move=>st'; rewrite findU c1 /=; case: ifP.
+    move/eqP=>Eq [Eq']; subst can_n stPm.
+    case Msg: (msg p)=>[|||b|||]; rewrite Msg in P;
+    do? by [NBlockMsg_dest_btChain q st p b Msg P H; move: (HHold _ F)].
+    by BlockMsg_dest q st b iF P Msg; move: (c3 (dst p) _ F)=>V;
+       move/eqP: (HHold _ F)=>Eq; subst can_bc;
+       rewrite (btExtend_seq_same V iB); by [|move: (HExt (dst p) _ F)].
+    by move=>_ F'; move: (HHold _ F').
+
+  (* can_bc is still the largest chain *)
+  + move=>n' bc'; rewrite/holds findU c1 /=; case: ifP.
+    move/eqP=>Eq st' [Eq']; subst n' stPm.
+    case Msg: (msg p)=>[|||b|||]; rewrite Msg in P;
+    do? by
+    [NBlockMsg_dest_btChain q st p b Msg P H=>Hc; move: (HGt (dst p) bc' _ F Hc)].
+    by BlockMsg_dest q st b iF P Msg; move: (c3 (dst p) _ F)=>V;
+       move/eqP=>Eq; subst bc';
+       (have: (has_chain (btChain (blockTree st)) st)
+          by rewrite/has_chain eqxx)=>O;
+       move: (HGt (dst p) (btChain (blockTree st)) _ F O)=>Gt;
+       move: (HExt (dst p) _ F)=>Ext;
+       move: (btExtend_seq_sameOrBetter_fref' V iB Gt Ext).
+    by move=>_ st' F'; move: (HGt n' bc' st' F').
+
+  (* clique topology is maintained *)
+  + move=>n' st'; rewrite findU c1 /=;
+    move: (HCliq (dst p) _ F)=>H1;
+    move: (step_nodes (Deliver Cw Al iF F P'))=>H2;
+    simplw w=>H3 _;
+    rewrite P in P'; rewrite P' /localState H3 in H2; clear P' H3.
+    case: ifP.
+    * move/eqP=>Eq [Eq']; subst n' stPm;
+      move=>z; specialize (H1 z); specialize (H2 z).
+      rewrite H2 in H1; move=>H3. specialize (H1 H3).
+      case Msg: (msg p)=>[|n prs|pr||||]; rewrite Msg in P;
+      rewrite [procMsg _ _ _] surjective_pairing in P; case: P=><- _;
+      destruct st; rewrite/procMsg/=; do? by [];
+      do? rewrite /Protocol.peers in H1.
+      by rewrite mem_undup mem_cat; apply/orP; left.
+      by case: ifP=>_;
+         [rewrite mem_undup|rewrite -cat1s mem_cat mem_undup; apply/orP; right].
+    * by move=>_ F'; clear H1; move: (HCliq n' _ F')=>H1;
+         move=>z; specialize (H1 z); specialize (H2 z);
+         rewrite H2 in H1=>H3; specialize (H1 H3).
+
+  (* applying conserved *)
+  + move=>n' st'; rewrite findU c1 /=; case: ifP; last first.
+    * move=>NDst F'; move: (HExt _ st' F')=>->.
+      rewrite/blocksFor{2}/inFlightMsgs.
+      admit.
+    * move/eqP=>Eq [Eq']; subst n' stPm.
+      case Msg: (msg p)=>[|||b|||]; rewrite Msg in P;
+      rewrite [procMsg _ _ _] surjective_pairing in P; case: P=>_ <-;
+      rewrite/blocksFor/inFlightMsgs; simplw w=>_ ->; rewrite/procMsg.
+      destruct st=>/=; case: ifP.
+      move=>_.
+
+   (*
+   (* conservation of blocks *)
+   split.
+   + rewrite!/holds!/localState=>n1 st1; rewrite findU c1 /=; case: ifP.
+     * move/eqP=>Eq [Eq']; subst n1 stPm.
+       move=>b iB1 n2 st2; rewrite findU c1 /=; case: ifP.
+        - by move/eqP=>Eq [Eq']; subst n2 st2; left.
+        - move=>X; simplw w=>-> _ F2.
+          case Msg: (msg p)=>[|||mb|||]; rewrite Msg in P;
+          rewrite [procMsg _ _ _] surjective_pairing in P; case: P=>P1 P2;
+          (* non-block msg => blockTree st1 = blockTree st *)
+          do? [
+            NBlockMsg_dest_bt q st p b' Msg H; rewrite Msg P1=>Eq;
+            rewrite -Eq in iB1; case: (HCon1 (dst p) _ F b iB1 n2 _ F2)=>[|biF]
+          ]; do? [by left]; do? [
+            right; rewrite/blocksFor/inFlightMsgs mem_undup; simplw w=>_ ->;
+            rewrite/blocksFor mem_undup in biF; move:biF; move/mapP=>[p'] H1 H2;
+            apply/mapP; exists p'; last done
+          ]; do? [
+            move: H1; rewrite mem_filter; move/andP=>[Dst] iF';
+            rewrite mem_filter in_rem_msg;
+            by [|rewrite Dst|
+                rewrite eq_sym in Dst; move/eqP in Dst; rewrite Dst in X;
+                move/eqP; move/eqP=>Eq'; subst p'; contradict X; rewrite eqxx
+            ]
+          ].
+          (* BlockMsg mb => blocktree st1 = btExtend (blockTree st) mb *)
+          move: (procMsg_block_btExtend_bt st mb (ts q)); rewrite P1=>Eq.
+          (* Is b something n1 just received (i.e. mb) or something it had? *)
+          rewrite Eq in iB1. move: (c3 (dst p) _ F)=>V.
+          Check btExtend_in_either.
+          have: (b = mb). admit. move=>E. subst mb.
+          move: (HCon2 p iF b Msg)=>[N] [St] [H1] H2.
+          specialize (H2 _ H1); simpl in H2.
+          move: (HCon1 N _ H1 b H2 n2 _ F2).
+
+
+
+          case Have: (mb ∈ (blockTree st)).
+          + move: (btExtend_withDup_noEffect Have)=>Eq'.
+            rewrite -Eq' in Eq; clear Eq'.
+            (* TODO: refactor to avoid duplication *)
+            rewrite Eq in iB1; case: (HCon1 (dst p) _ F b iB1 n2 _ F2)=>[|biF].
+            by left.
+            right; rewrite/blocksFor/inFlightMsgs mem_undup; simplw w=>_ ->;
+            rewrite/blocksFor mem_undup in biF; move:biF; move/mapP=>[p'] H1 H2;
+            apply/mapP; exists p'; last done.
+            move: H1; rewrite mem_filter; move/andP=>[Dst] iF';
+                rewrite mem_filter in_rem_msg;
+                by [|rewrite Dst|
+                    rewrite eq_sym in Dst; move/eqP in Dst; rewrite Dst in X;
+                    move/eqP; move/eqP=>Eq'; subst p'; contradict X; rewrite eqxx
+            ].
+          + case Eq': (b == mb).
+            move/eqP in Eq'; subst b.
+            move: (HCon2 p iF mb Msg)=>[N] [St] [H1] H2.
+            specialize (H2 _ H1); simpl in H2.
+            case: (HCon1 N _ H1 mb H2 n2 _ F2).
+    *)
